src/NLustre/DupRegRem/DRR.v
@@ -1,0 +1,67 @@
+From Velus Require Import Common.
+From Velus Require Import Operators.
+From Velus Require Import Clocks.
+From Velus Require Import IndexedStreams.
+From Velus Require Import CommonTyping.
+
+From Velus Require Import CoreExpr.CoreExpr.
+From Velus Require Export NLustre.NLSyntax.
+From Velus Require Export NLustre.IsDefined.
+From Velus Require Export NLustre.Memories.
+From Velus Require Export NLustre.NLIndexedSemantics.
+From Velus Require Export NLustre.NLOrdered.
+From Velus Require Export NLustre.NLClocking.
+From Velus Require Export NLustre.NLTyping.
+From Velus Require Export NLustre.NLNormalArgs.
+From Velus Require Export NLustre.DupRegRem.DupRegRem.
+From Velus Require Export NLustre.DupRegRem.DRRTyping.
+From Velus Require Export NLustre.DupRegRem.DRRClocking.
+From Velus Require Export NLustre.DupRegRem.DRRNormalArgs.
+From Velus Require Export NLustre.DupRegRem.DRRCorrectness.
+
+Module Type DRR
+       (Ids   : IDS)
+       (Op    : OPERATORS)
+       (OpAux : OPERATORS_AUX Ids Op)
+       (ComTyp: COMMONTYPING Ids Op OpAux)
+       (Cks   : CLOCKS Ids Op OpAux)
+       (IStr  : INDEXEDSTREAMS Ids Op OpAux Cks)
+       (CE    : COREEXPR Ids Op OpAux ComTyp Cks IStr)
+       (Syn   : NLSYNTAX Ids Op OpAux Cks CE.Syn)
+       (Ord   : NLORDERED Ids Op OpAux Cks CE.Syn Syn)
+       (Typ   : NLTYPING Ids Op OpAux Cks CE.Syn Syn Ord CE.Typ)
+       (Norm  : NLNORMALARGS Ids Op OpAux Cks CE.Syn CE.Typ Syn Ord Typ)
+       (Mem   : MEMORIES Ids Op OpAux Cks CE.Syn Syn)
+       (IsD   : ISDEFINED Ids Op OpAux Cks CE.Syn Syn Mem)
+       (Clo   : NLCLOCKING Ids Op OpAux Cks CE.Syn Syn Ord Mem IsD CE.Clo)
+       (Sem   : NLINDEXEDSEMANTICS Ids Op OpAux Cks CE.Syn Syn IStr Ord CE.Sem).
+  Declare Module Export DupRegRem  : DUPREGREM            Ids Op OpAux Cks CE.Syn Syn.
+  Declare Module Export DRRTyp     : DRRTYPING            Ids Op OpAux Cks CE.Syn CE.Typ Syn Ord Typ DupRegRem.
+  Declare Module Export DRRClo     : DRRCLOCKING          Ids Op OpAux Cks CE.Syn CE.Clo Syn Ord Mem IsD Clo DupRegRem.
+  Declare Module Export DRRNorm    : DRRNORMALARGS        Ids Op OpAux Cks CE.Syn CE.Typ Syn Ord Typ Norm DupRegRem.
+  Declare Module Export DRRCor     : DRRCORRECTNESS       Ids Op OpAux Cks IStr CE.Syn CE.Sem Syn Ord Sem DupRegRem.
+End DRR.
+
+Module DRRFun
+       (Ids   : IDS)
+       (Op    : OPERATORS)
+       (OpAux : OPERATORS_AUX Ids Op)
+       (ComTyp: COMMONTYPING Ids Op OpAux)
+       (Cks   : CLOCKS Ids Op OpAux)
+       (IStr  : INDEXEDSTREAMS Ids Op OpAux Cks)
+       (CE    : COREEXPR Ids Op OpAux ComTyp Cks IStr)
+       (Syn   : NLSYNTAX Ids Op OpAux Cks CE.Syn)
+       (Ord   : NLORDERED Ids Op OpAux Cks CE.Syn Syn)
+       (Typ   : NLTYPING Ids Op OpAux Cks CE.Syn Syn Ord CE.Typ)
+       (Norm  : NLNORMALARGS Ids Op OpAux Cks CE.Syn CE.Typ Syn Ord Typ)
+       (Mem   : MEMORIES Ids Op OpAux Cks CE.Syn Syn)
+       (IsD   : ISDEFINED Ids Op OpAux Cks CE.Syn Syn Mem)
+       (Clo   : NLCLOCKING Ids Op OpAux Cks CE.Syn Syn Ord Mem IsD CE.Clo)
+       (Sem   : NLINDEXEDSEMANTICS Ids Op OpAux Cks CE.Syn Syn IStr Ord CE.Sem)
+       <: DRR Ids Op OpAux ComTyp Cks IStr CE Syn Ord Typ Norm Mem IsD Clo Sem.
+  Module Export DupRegRem  := DupRegRemFun            Ids Op OpAux Cks CE.Syn Syn.
+  Module Export DRRTyp     := DrrTypingFun            Ids Op OpAux Cks CE.Syn CE.Typ Syn Ord Typ DupRegRem.
+  Module Export DRRClo     := DrrClockingFun          Ids Op OpAux Cks CE.Syn CE.Clo Syn Ord Mem IsD Clo DupRegRem.
+  Module Export DRRNorm    := DrrNormalArgsFun        Ids Op OpAux Cks CE.Syn CE.Typ Syn Ord Typ Norm DupRegRem.
+  Module Export DRRCor     := DrrCorrectnessFun       Ids Op OpAux Cks IStr CE.Syn CE.Sem Syn Ord Sem DupRegRem.
+End DRRFun.
